theories/Operational/Common/OSLocalAdapterContract.v
@@ -1,0 +1,159 @@
+From RocqSched Require Import Foundation.Base.
+From RocqSched Require Import Semantics.Schedule.
+From RocqSched Require Import Multicore.Common.MultiCoreBase.
+From RocqSched Require Import Multicore.Common.Admissibility.
+From RocqSched Require Import Operational.Common.State.
+From RocqSched Require Import Operational.Common.Step.
+From RocqSched Require Import Operational.Common.OSProjectionInterface.
+From RocqSched Require Import Operational.Common.ConcreteExecution.
+From RocqSched Require Import Operational.Common.Projection.
+From RocqSched Require Import Operational.Common.ProjectionInvariants.
+
+(* Local adapter-side contract over individual projected steps. This keeps the
+   global projection packages reusable while letting concrete adapters justify
+   the projection with event-local obligations. *)
+Record local_labeled_concrete_projection_sound
+    {CState : Type}
+    {P : OSLabeledProjection CState}
+    (jobs : JobId -> Job)
+    (m : nat)
+    (ex : labeled_concrete_execution P m) : Prop :=
+  mkLocalLabeledConcreteProjectionSound {
+    llcps_init_release :
+      forall c j,
+        c < m ->
+        op_current
+          (os_to_op_state (osl_to_os_projection P) (lce_trace ex 0))
+          c = Some j ->
+        released jobs j 0;
+    llcps_init_completion :
+      forall c j,
+        c < m ->
+        op_current
+          (os_to_op_state (osl_to_os_projection P) (lce_trace ex 0))
+          c = Some j ->
+        ~ completed
+            jobs
+            m
+            (project_schedule (osl_to_op_trace P (lce_trace ex)))
+            j 0;
+    llcps_current_origin :
+      forall t c j,
+        c < m ->
+        op_current
+          (os_to_op_state (osl_to_os_projection P) (lce_trace ex (S t)))
+          c = Some j ->
+        op_current
+          (os_to_op_state (osl_to_os_projection P) (lce_trace ex t))
+          c = Some j \/
+        os_step_label P (lce_trace ex t) (lce_trace ex (S t)) = EvDispatch c j \/
+        exists old,
+          os_step_label P (lce_trace ex t) (lce_trace ex (S t)) =
+          EvPreempt c old j;
+    llcps_dispatch_release :
+      forall t c j,
+        c < m ->
+        os_step_label P (lce_trace ex t) (lce_trace ex (S t)) = EvDispatch c j ->
+        released jobs j (S t);
+    llcps_persistent_completion :
+      forall t c j,
+        c < m ->
+        op_current
+          (os_to_op_state (osl_to_os_projection P) (lce_trace ex t))
+          c = Some j ->
+        op_current
+          (os_to_op_state (osl_to_os_projection P) (lce_trace ex (S t)))
+          c = Some j ->
+        ~ completed
+            jobs
+            m
+            (project_schedule (osl_to_op_trace P (lce_trace ex)))
+            j (S t);
+    llcps_dispatch_completion :
+      forall t c j,
+        c < m ->
+        os_step_label P (lce_trace ex t) (lce_trace ex (S t)) = EvDispatch c j ->
+        ~ completed
+            jobs
+            m
+            (project_schedule (osl_to_op_trace P (lce_trace ex)))
+            j (S t);
+    llcps_preempt_release :
+      forall t c old new,
+        c < m ->
+        os_step_label P (lce_trace ex t) (lce_trace ex (S t)) =
+        EvPreempt c old new ->
+        released jobs new (S t);
+    llcps_preempt_completion :
+      forall t c old new,
+        c < m ->
+        os_step_label P (lce_trace ex t) (lce_trace ex (S t)) =
+        EvPreempt c old new ->
+        ~ completed
+            jobs
+            m
+            (project_schedule (osl_to_op_trace P (lce_trace ex)))
+            new (S t);
+  }.
+
+Record local_labeled_concrete_multicore_projection_sound
+    {CState : Type}
+    {P : OSLabeledProjection CState}
+    (jobs : JobId -> Job)
+    (adm : admissible_cpu)
+    (m : nat)
+    (ex : labeled_concrete_execution P m) : Prop :=
+  mkLocalLabeledConcreteMulticoreProjectionSound {
+    llcmps_projection_sound :
+      local_labeled_concrete_projection_sound jobs m ex;
+    llcmps_idle_outside :
+      forall t,
+        op_idle_outside_range
+          m
+          (os_to_op_state (osl_to_os_projection P) (lce_trace ex t));
+    llcmps_placement :
+      forall t,
+        op_respects_admissibility
+          adm
+          m
+          (os_to_op_state (osl_to_os_projection P) (lce_trace ex t));
+  }.
+
+Record os_local_multicore_adapter_contract
+    {CState : Type}
+    (P : OSLabeledProjection CState)
+    (jobs : JobId -> Job)
+    (adm : admissible_cpu)
+    (m : nat) : Type :=
+  mkOSLocalMulticoreAdapterContract {
+    olac_execution : labeled_concrete_execution P m;
+    olac_sound :
+      local_labeled_concrete_multicore_projection_sound jobs adm m olac_execution;
+  }.
+
+Arguments llcps_init_release
+  {CState P jobs m ex} _ _ _ _ _.
+Arguments llcps_init_completion
+  {CState P jobs m ex} _ _ _ _ _.
+Arguments llcps_current_origin
+  {CState P jobs m ex} _ _ _ _ _ _.
+Arguments llcps_dispatch_release
+  {CState P jobs m ex} _ _ _ _ _.
+Arguments llcps_persistent_completion
+  {CState P jobs m ex} _ _ _ _ _ _.
+Arguments llcps_dispatch_completion
+  {CState P jobs m ex} _ _ _ _ _.
+Arguments llcps_preempt_release
+  {CState P jobs m ex} _ _ _ _ _ _.
+Arguments llcps_preempt_completion
+  {CState P jobs m ex} _ _ _ _ _ _.
+Arguments llcmps_projection_sound
+  {CState P jobs adm m ex} _.
+Arguments llcmps_idle_outside
+  {CState P jobs adm m ex} _ _.
+Arguments llcmps_placement
+  {CState P jobs adm m ex} _ _.
+Arguments olac_execution
+  {CState P jobs adm m} _.
+Arguments olac_sound
+  {CState P jobs adm m} _.
